sha3/proof/old/SLCommon.ec
@@ -1,0 +1,208 @@
+
+(** This is a theory for the Squeezeless sponge: where the ideal
+    functionality is a fixed-output-length random oracle whose output
+    length is the input block size. We prove its security even when
+    padding is not prefix-free. **)
+require import Pred Fun Option Pair Int Real StdOrder Ring.
+require import List FSet NewFMap Utils Common.
+
+require (*..*) RndOrcl Indifferentiability.
+(*...*) import Dprod Dexcepted Capacity IntOrder.
+
+type state  = block  * capacity.
+op   dstate = bdistr * cdistr.
+
+
+clone include Indifferentiability with
+  type p     <- state, 
+  type f_in  <- block list,
+  type f_out <- block
+  rename [module] "GReal" as "RealIndif"
+         [module] "GIdeal"  as "IdealIndif".
+
+
+(** max number of call to the permutation and its inverse, 
+    including those performed by the construction. *)
+op max_size : int.
+
+(** Ideal Functionality **)
+clone export Tuple as TupleBl with
+  type t <- block,
+  op Support.enum <- Block.words
+  proof Support.enum_spec by exact Block.enum_spec. 
+
+op bl_enum = flatten (mkseq (fun i => wordn i) (max_size + 1)). 
+op bl_univ = FSet.oflist bl_enum.
+
+clone RndOrcl as RndOrclB with 
+  type from <- block list,
+  type to   <- block.
+ 
+clone export RndOrclB.RestrIdeal as Functionality with
+  op sample _ <- bdistr,
+  op test l   <- List.size l <= max_size,
+  op univ     <- bl_univ,
+  op dfl      <- b0
+  proof *.
+realize sample_ll by exact Block.DWord.bdistr_ll.
+realize testP.
+proof.
+  move=> x; rewrite mem_oflist-flattenP; split=>[_|[s[/mkseqP[i[/=_->>]]/wordnP->/#]]].
+  exists (wordn (size x));cut Hsx := size_ge0 x.
+  rewrite wordnP max_ler //= mkseqP /=;exists (size x);smt ml=0.
+qed.
+
+(** We can now define the squeezeless sponge construction **)
+module SqueezelessSponge (P:PRIMITIVE): CONSTRUCTION(P), FUNCTIONALITY = {
+  proc init () = {} 
+
+  proc f(p : block list): block = {
+    var (sa,sc) <- (b0,c0);
+
+    if (1 <= size p /\ p <> [b0]) {
+      while (p <> []) { (* Absorption *)
+        (sa,sc) <@ P.f((sa +^ head witness p,sc));
+        p <- behead p;
+      }
+    }
+    return sa;          (* Squeezing phase (non-iterated) *)
+  }
+}.
+
+clone export Pair.Dprod.Sample as Sample2 with 
+  type t1 <- block,
+  type t2 <- capacity,
+  op d1   <- bdistr,
+  op d2   <- cdistr.
+
+(* -------------------------------------------------------------------------- *)
+(** TODO move this **)
+
+op incl (m m':('a,'b)fmap) = 
+  forall x,  m .[x] <> None => m'.[x] = m.[x].
+
+(* -------------------------------------------------------------------------- *)
+(** usefull type and operators for the proof **)
+
+type caller = [ I | D ].
+
+type handle  = int.
+
+type hstate = block * handle.
+ 
+type ccapacity = capacity * caller.
+
+type smap    = (state , state    ) fmap.
+type hsmap   = (hstate, hstate   ) fmap.
+type handles = (handle, ccapacity) fmap.
+
+(* Did we use it? *)
+op (<=) (o1 o2 : caller) = o1 = I \/ o2 = D.
+
+(* Did we use it? *)
+op max (o1 o2 : caller) =
+  with o1 = I => o2
+  with o1 = D => D.
+
+pred is_pre_permutation (m mi : ('a,'a) fmap) =
+     (forall x, mem (rng m) x => mem (dom mi) x)
+  /\ (forall x, mem (rng mi) x => mem (dom m) x).
+
+lemma half_permutation_set (m' mi' : ('a,'a) fmap) x' y':
+     (forall x, mem (rng m') x => mem (dom mi') x)
+  => (forall x, mem (rng m'.[x' <- y']) x => mem (dom mi'.[y' <- x']) x).
+proof.
+  move=> h x0.
+  rewrite rng_set domP !in_fsetU in_fset1 => [/rng_rem_le in_rng|//=].
+  by rewrite h.
+qed.
+
+lemma pre_permutation_set (m mi : ('a,'a) fmap) x y:
+  is_pre_permutation m mi =>
+  is_pre_permutation m.[x <- y] mi.[y <- x].
+proof.
+  move=> [dom_mi dom_m].
+  by split; apply/half_permutation_set.
+qed.    
+
+(** Operators and properties of handles *)
+
+op hinv (handles:handles) (c:capacity) = 
+   find (fun _ => pred1 c \o fst) handles.
+
+op hinvD (handles:handles) (c:capacity) = 
+   find (fun _ => pred1 (c,D)) handles.
+
+op huniq (handles:handles) = 
+  forall h1 h2 cf1 cf2, 
+     handles.[h1] = Some cf1 => 
+     handles.[h2] = Some cf2 => 
+     cf1.`1 = cf2.`1 => h1 = h2.
+
+lemma hinvP handles c:
+  if hinv handles c = None then forall h f, handles.[h] <> Some(c,f)
+  else exists f, handles.[oget (hinv handles c)] = Some(c,f).
+proof.
+  cut @/pred1@/(\o)/=[[h []->[]Hmem <<-]|[]->H h f]/= := 
+    findP (fun (_ : handle) => pred1 c \o fst) handles.
+  + by exists (oget handles.[h]).`2;rewrite oget_some get_oget;2:case (oget handles.[h]).
+  by rewrite -not_def=> Heq; cut := H h;rewrite in_dom Heq.
+qed.
+
+lemma huniq_hinv (handles:handles) (h:handle): 
+  huniq handles => mem (dom handles) h => hinv handles (oget handles.[h]).`1 = Some h.
+proof.
+  move=> Huniq;pose c := (oget handles.[h]).`1.
+  cut:=Huniq h;cut:=hinvP handles c.
+  case (hinv _ _)=> /=[Hdiff _| h' +/(_ h')];1:by rewrite in_dom /#.
+  by move=> [f ->] /(_ (oget handles.[h]) (c,f)) H1 H2;rewrite H1 // get_oget.
+qed.
+
+lemma hinvDP handles c:
+  if hinvD handles c = None then forall h, handles.[h] <> Some(c,D)
+  else handles.[oget (hinvD handles c)] = Some(c,D).
+proof.
+  cut @/pred1/=[[h []->[]Hmem ]|[]->H h ]/= := 
+    findP (fun (_ : handle) => pred1 (c,D)) handles.
+  + by rewrite oget_some get_oget.
+  by rewrite -not_def=> Heq; cut := H h;rewrite in_dom Heq. 
+qed.
+
+lemma huniq_hinvD (handles:handles) c: 
+  huniq handles => mem (rng handles) (c,D) => handles.[oget (hinvD handles c)] = Some(c,D).
+proof.
+  move=> Huniq;rewrite in_rng=> [h]H;case: (hinvD _ _) (Huniq h) (hinvDP handles c)=>//=.
+  by move=>_/(_ h);rewrite H.
+qed.
+
+lemma huniq_hinvD_h h (handles:handles) c: 
+  huniq handles => handles.[h] = Some (c,D) => hinvD handles c = Some h.
+proof.
+  move=> Huniq;case: (hinvD _ _) (hinvDP handles c)=>/= [H|h'];1: by apply H. 
+  by rewrite oget_some=> /Huniq H/H. 
+qed.
+
+(* Functionnal version of the construction using handle *)
+
+op step_hpath (mh:hsmap) (sah:hstate option) (b:block) = 
+    if sah = None then None 
+    else 
+      let sah = oget sah in 
+      mh.[(sah.`1 +^ b, sah.`2)].
+
+op build_hpath (mh:hsmap) (bs:block list) = 
+   foldl (step_hpath mh) (Some (b0,0)) bs.
+
+lemma build_hpathP mh p v h: 
+  build_hpath mh p = Some (v, h) =>
+  (p = [] /\ v=b0 /\ h=0) \/ 
+  exists p' b v' h',  
+    p = rcons p' b /\ build_hpath mh p' = Some(v',h') /\ mh.[(v'+^b, h')] = Some(v,h).
+proof.
+  elim/last_ind:p=>@/build_hpath //= p' b _. 
+  rewrite -cats1 foldl_cat /= => H;right;exists p',b. 
+  move:H;rewrite {1}/step_hpath;case (foldl _ _ _)=> //= -[v' h'].
+  by rewrite oget_some /==>Heq; exists v',h';rewrite -cats1.
+qed.
+
+
